otway-rees-fixed/OYRS.Protocol.fst
@@ -32,6 +32,7 @@ let install_sk_at_auth_server #i #us srv p sk =
 
   new_session #oyrs_preds #now srv new_sess_idx 0 ser_st
 
+#push-options "--z3rlimit 300"
 let initiator_send_msg_1 a a_si =
   // get initiator session
   let now = global_timestamp () in
@@ -41,17 +42,19 @@ let initiator_send_msg_1 a a_si =
   | Success (InitiatorInit srv k_as b) -> (
     // generate conversation id and initiator nonce
     let (|_,c|) = rand_gen #oyrs_preds public (nonce_usage "conv_id") in
-    let (|_,n_a|) = rand_gen #oyrs_preds (readers [P a; P srv]) (nonce_usage "nonce_i") in
+    let (|now,n_a|) = rand_gen #oyrs_preds (readers [P a; P srv]) (nonce_usage "nonce_i") in
 
     // trigger event 'initiate'
-    let event = event_initiate c a b n_a in
+    let event = event_initiate c a b srv n_a in
     trigger_event #oyrs_preds a event;
 
     // create and send first message
     let ev1 = EncMsg1 c a b n_a in
     let now = global_timestamp () in
     let (|tag_ev1,ser_ev1|) = serialize_encval now ev1 (get_label oyrs_key_usages k_as) in
-    let c_ev1 = aead_enc #oyrs_global_usage #now #(get_label oyrs_key_usages k_as) k_as (string_to_bytes #oyrs_global_usage #now "iv") ser_ev1 (string_to_bytes #oyrs_global_usage #now "ev_i") in
+    assert(tag_ev1 = "ev1");
+    parse_serialize_encval_lemma now ev1 (get_label oyrs_key_usages k_as);
+    let c_ev1 = aead_enc #oyrs_global_usage #now #(get_label oyrs_key_usages k_as) k_as (string_to_bytes #oyrs_global_usage #now "iv") ser_ev1 (string_to_bytes #oyrs_global_usage #now "ev1") in
 
     let msg1:message now = Msg1 c a b (|tag_ev1,c_ev1|) in
     let ser_msg1 = serialize_msg now msg1 in
@@ -88,14 +91,16 @@ let responder_send_msg_2 b msg1_idx b_si =
         let (|_,n_b|) = rand_gen #oyrs_preds (readers [P b; P srv]) (nonce_usage "nonce_r") in
 
         // trigger event 'request key'
-        let event = event_request_key c a b n_b in
+        let event = event_request_key c a b srv n_b in
         trigger_event #oyrs_preds b event;
 
         // create and send second message
         let ev2 = EncMsg2 c a b n_b in
         let now = global_timestamp () in
         let (|tag_ev2,ser_ev2|) = serialize_encval now ev2 (get_label oyrs_key_usages k_bs) in
-        let c_ev2 = aead_enc #oyrs_global_usage #now #(get_label oyrs_key_usages k_bs) k_bs (string_to_bytes #oyrs_global_usage #now "iv") ser_ev2 (string_to_bytes #oyrs_global_usage #now "ev_r") in
+        assert(tag_ev2 = "ev2");
+        parse_serialize_encval_lemma now ev2 (get_label oyrs_key_usages k_bs);
+        let c_ev2 = aead_enc #oyrs_global_usage #now #(get_label oyrs_key_usages k_bs) k_bs (string_to_bytes #oyrs_global_usage #now "iv") ser_ev2 (string_to_bytes #oyrs_global_usage #now "ev2") in
 
         let c_ev_a:msg oyrs_global_usage now public = c_ev_a in
         let msg2:message now = Msg2 c a b (|tag_ev_a,c_ev_a|) (|tag_ev2,c_ev2|) in
@@ -132,7 +137,6 @@ let find_auth_server_session_helper (svr:principal) (p:principal) :
   )
   | None -> error ("find_auth_server_session_helper: no session for " ^ p ^ " found")
 
-#push-options "--z3rlimit 200"
 let server_send_msg_3 srv msg2_idx =
   // receive and parse second message
   let (|now,b,ser_msg2|) = receive_i #oyrs_preds msg2_idx srv in
@@ -148,10 +152,10 @@ let server_send_msg_3 srv msg2_idx =
 
       // decrypt parts of message encrypted by initiator and responder, respectively
       let c_ev_a:msg oyrs_global_usage now public = c_ev_a in
-      match aead_dec #oyrs_global_usage #now #(get_label oyrs_key_usages k_as) k_as (string_to_bytes #oyrs_global_usage #now "iv") c_ev_a (string_to_bytes #oyrs_global_usage #now "ev_i") with
+      match aead_dec #oyrs_global_usage #now #(get_label oyrs_key_usages k_as) k_as (string_to_bytes #oyrs_global_usage #now "iv") c_ev_a (string_to_bytes #oyrs_global_usage #now "ev1") with
       | Success ser_ev_a -> (
         let c_ev_b:msg oyrs_global_usage now public = c_ev_b in
-        match aead_dec #oyrs_global_usage #now #(get_label oyrs_key_usages k_bs) k_bs (string_to_bytes #oyrs_global_usage #now "iv") c_ev_b (string_to_bytes #oyrs_global_usage #now "ev_r") with
+        match aead_dec #oyrs_global_usage #now #(get_label oyrs_key_usages k_bs) k_bs (string_to_bytes #oyrs_global_usage #now "iv") c_ev_b (string_to_bytes #oyrs_global_usage #now "ev2") with
         | Success ser_ev_b -> (
           // parse the decrypted message parts
           let tagged_ser_ev_a:ser_encval now (get_label oyrs_key_usages k_as) = (|tag_ev_a,ser_ev_a|) in
@@ -170,30 +174,41 @@ let server_send_msg_3 srv msg2_idx =
               else
                 // generate shared conversation key between initiator and responder
                 let prev = now in
-                let (|now,k_ab|) = rand_gen #oyrs_preds (readers [P srv; P a; P b]) (aead_usage "sk_i_r") in
+                let (|_,k_ab|) = rand_gen #oyrs_preds (readers [P srv; P a; P b]) (aead_usage "sk_i_r") in
 
                 // trigger event 'send key'
-                let event = event_send_key c a b n_a n_b k_ab in
+                let event = event_send_key c a b srv n_a n_b k_ab in
                 trigger_event #oyrs_preds srv event;
 
                 // create and send third message
-                let ev3_i = EncMsg3_I n_a k_ab in
+                let ev3_i = EncMsg3_I n_a b k_ab in
+                let now = global_timestamp () in
                 can_flow_later prev now (readers [P a; P srv]) (readers [P a; P srv]);
                 includes_can_flow_lemma now [P srv; P a; P b] [P a; P srv];
                 assert(is_msg oyrs_global_usage now k_ab (get_label oyrs_key_usages k_as));
                 assert(is_msg oyrs_global_usage prev n_a (get_label oyrs_key_usages k_as));
                 assert(is_msg oyrs_global_usage now n_a (get_label oyrs_key_usages k_as));
                 let (|tag_ev3_i,ser_ev3_i|) = serialize_encval now ev3_i (get_label oyrs_key_usages k_as) in
-                let c_ev3_i = aead_enc #oyrs_global_usage #now #(get_label oyrs_key_usages k_as) k_as (string_to_bytes #oyrs_global_usage #now "iv") ser_ev3_i (string_to_bytes #oyrs_global_usage #now "ev_i") in
+                let ad = (string_to_bytes #oyrs_global_usage #now "ev3_i") in
+                assert(tag_ev3_i = "ev3_i");
+                assert(was_rand_generated_before now k_ab (readers [P srv; P a; P b]) (aead_usage "sk_i_r"));
+                assert(did_event_occur_before now srv (event_send_key c a b srv n_a n_b k_ab));
+                parse_serialize_encval_lemma now ev3_i (get_label oyrs_key_usages k_as);
+                assert(can_aead_encrypt now "sk_i_srv" k_as (|tag_ev3_i,ser_ev3_i|) ad);
+                let c_ev3_i = aead_enc #oyrs_global_usage #now #(get_label oyrs_key_usages k_as) k_as (string_to_bytes #oyrs_global_usage #now "iv") ser_ev3_i ad in
 
-                let ev3_r = EncMsg3_R n_b k_ab in
+                let ev3_r = EncMsg3_R n_b a k_ab in
                 can_flow_later prev now (readers [P b; P srv]) (readers [P b; P srv]);
                 includes_can_flow_lemma now [P srv; P a; P b] [P b; P srv];
                 assert(is_msg oyrs_global_usage now k_ab (get_label oyrs_key_usages k_bs));
                 assert(is_msg oyrs_global_usage prev n_b (get_label oyrs_key_usages k_bs));
                 assert(is_msg oyrs_global_usage now n_b (get_label oyrs_key_usages k_bs));
                 let (|tag_ev3_r,ser_ev3_r|) = serialize_encval now ev3_r (get_label oyrs_key_usages k_bs) in
-                let c_ev3_r = aead_enc #oyrs_global_usage #now #(get_label oyrs_key_usages k_bs) k_bs (string_to_bytes #oyrs_global_usage #now "iv") ser_ev3_r (string_to_bytes #oyrs_global_usage #now "ev_r") in
+                let ad = (string_to_bytes #oyrs_global_usage #now "ev3_r") in
+                assert(tag_ev3_r = "ev3_r");
+                parse_serialize_encval_lemma now ev3_r (get_label oyrs_key_usages k_bs);
+                assert(can_aead_encrypt now "sk_r_srv" k_bs (|tag_ev3_r,ser_ev3_r|) ad);
+                let c_ev3_r = aead_enc #oyrs_global_usage #now #(get_label oyrs_key_usages k_bs) k_bs (string_to_bytes #oyrs_global_usage #now "iv") ser_ev3_r ad in
 
                 let msg3:message now = Msg3 c (|tag_ev3_i,c_ev3_i|) (|tag_ev3_r,c_ev3_r|) in
                 let ser_msg3 = serialize_msg now msg3 in
@@ -251,7 +266,6 @@ let server_send_msg_3 srv msg2_idx =
       | Error e -> error ("srv_send_m3: decryption of initiator part failed: " ^ e)
   )
   | _ -> error "srv_send_m3: wrong message\n"
-#pop-options
 
 let responder_send_msg_4 b msg3_idx b_si =
   // get responder session
@@ -272,19 +286,59 @@ let responder_send_msg_4 b msg3_idx b_si =
         else
           // decrypt part of message intended for responder
           let now = global_timestamp () in
-          match aead_dec #oyrs_global_usage #now #(get_label oyrs_key_usages k_bs) k_bs (string_to_bytes #oyrs_global_usage #now "iv") c_ev_b (string_to_bytes #oyrs_global_usage #now "ev_r") with
+          let ad = (string_to_bytes #oyrs_global_usage #now "ev3_r") in
+          match aead_dec #oyrs_global_usage #now #(get_label oyrs_key_usages k_bs) k_bs (string_to_bytes #oyrs_global_usage #now "iv") c_ev_b ad with
           | Success ser_ev_b -> (
             // parse the decrypted part
             let tagged_ser_ev_b:ser_encval now (get_label oyrs_key_usages k_bs) = (|tag_ev_b,ser_ev_b|) in
             match parse_encval tagged_ser_ev_b with
-            | Success (EncMsg3_R n_b' k_ab) -> (
+            | Success (EncMsg3_R n_b' a' k_ab) -> (
               parsed_encval_is_valid_lemma tagged_ser_ev_b;
 
               if n_b <> n_b' then error "r_send_m4: responder nonce in message does not match with the stored nonce\n"
+              else if a <> a' then error "r_send_m4: stored initiator does not match with initiator in part encrypted for responder\n"
               else
                 // trigger event 'forward key'
+                // k_bs readers corrupted ?
+                publishable_readers_implies_corruption #now [P b; P srv];
+                // readers corrupted or aead pred holds
+                assert(is_publishable oyrs_global_usage now k_bs
+                  \/ aead_pred oyrs_usage_preds now "sk_r_srv" k_bs ser_ev_b ad);
+
+                // if aead pred holds, can aead encrypt from usage preds holds for earlier ts
+                assert(aead_pred oyrs_usage_preds now "sk_r_srv" k_bs ser_ev_b ad
+                  ==> (exists i. later_than now i /\ oyrs_usage_preds.can_aead_encrypt i "sk_r_srv" k_bs ser_ev_b ad));
+                assert(aead_pred oyrs_usage_preds now "sk_r_srv" k_bs ser_ev_b ad
+                  ==> (exists i. later_than now i /\ oyrs_aead_pred i "sk_r_srv" k_bs ser_ev_b ad));
+                // plug in definition of can aead encrypt from usage preds
+                assert(exists i. (later_than now i /\ oyrs_aead_pred i "sk_r_srv" k_bs ser_ev_b ad)
+                  ==> (forall (t:string{CryptoLib.bytes_to_string ad = Success t}). can_aead_encrypt i "sk_r_srv" k_bs (|t,ser_ev_b|) ad));
+                assert(aead_pred oyrs_usage_preds now "sk_r_srv" k_bs ser_ev_b ad
+                  ==> (exists i. forall (t:string{CryptoLib.bytes_to_string ad = Success t}). later_than now i /\ can_aead_encrypt i "sk_r_srv" k_bs (|t,ser_ev_b|) ad)); // implication transitive step 1
+
+                assert(tag_ev_b = "ev3_r");
+
+                // all strings t -> associated tag
+                can_aead_encrypt_encval_lemma now tag_ev_b (get_label oyrs_key_usages k_bs) "sk_r_srv" k_bs ser_ev_b ad;
+                assert(exists i. forall (t:string{CryptoLib.bytes_to_string ad = Success t}). (later_than now i /\ can_aead_encrypt i "sk_r_srv" k_bs (|t,ser_ev_b|) ad)
+                  ==> can_aead_encrypt i "sk_r_srv" k_bs (|tag_ev_b,ser_ev_b|) ad);
+                assert(aead_pred oyrs_usage_preds now "sk_r_srv" k_bs ser_ev_b ad
+                  ==> (exists i. later_than now i /\ can_aead_encrypt i "sk_r_srv" k_bs (|tag_ev_b,ser_ev_b|) ad)); // implication transitive step 2
+                assert(exists i. (later_than now i /\ can_aead_encrypt i "sk_r_srv" k_bs (|tag_ev_b,ser_ev_b|) ad)
+                  ==> (exists c n_a. did_event_occur_before i srv (event_send_key c a b srv n_a n_b k_ab)));
+                assert(aead_pred oyrs_usage_preds now "sk_r_srv" k_bs ser_ev_b ad
+                  ==> (exists i c n_a. later_than now i /\ did_event_occur_before i srv (event_send_key c a b srv n_a n_b k_ab))); // implication transitive step 3
+                assert(exists i c n_a. later_than now i /\ did_event_occur_before i srv (event_send_key c a b srv n_a n_b k_ab)
+                  ==> did_event_occur_before now srv (event_send_key c a b srv n_a n_b k_ab));
+
+                // implication transitive
+                assert(aead_pred oyrs_usage_preds now "sk_r_srv" k_bs ser_ev_b ad
+                  ==> (exists c n_a. did_event_occur_before now srv (event_send_key c a b srv n_a n_b k_ab)));
+                // substitute aead pred with implication
+                assert(is_publishable oyrs_global_usage now k_bs \/ (exists c n_a. did_event_occur_before now srv (event_send_key c a b srv n_a n_b k_ab)));
+                assert((exists c n_a. did_event_occur_before now srv (event_send_key c a b srv n_a n_b k_ab)) \/ (corrupt_id now (P srv)) \/ (corrupt_id now (P b)));
                 let prev = now in
-                let event = event_forward_key c a b k_ab in
+                let event = event_forward_key c a b srv k_ab in
                 trigger_event #oyrs_preds b event;
 
                 // create and send fourth message
@@ -309,6 +363,8 @@ let responder_send_msg_4 b msg3_idx b_si =
                 includes_can_flow_lemma now [P b; P srv] [P b];
                 can_flow_transitive now (get_label oyrs_key_usages k_ab) (readers [P b; P srv]) (readers [P b]);
                 assert(is_msg oyrs_global_usage now k_ab (readers [P b]));
+                // prev -> now
+                assert(can_aead_encrypt prev "sk_r_srv" k_bs tagged_ser_ev_b ad ==> (exists p. was_rand_generated_before prev k_ab (readers [P srv; P p; P b]) (aead_usage "sk_i_r")));
                 let ser_st = serialize_session_st now b b_si b_vi st_r_sent_m4 in
                 update_session #oyrs_preds #now b b_si b_vi ser_st;
 
@@ -353,7 +409,7 @@ let initiator_recv_msg_4 a msg4_idx a_si =
               else
                 // trigger event 'recv key'
                 let prev = now in
-                let event = event_recv_key c a b k_ab in
+                let event = event_recv_key c a b srv k_ab in
                 trigger_event #oyrs_preds a event;
 
                 // update initiator session
@@ -384,3 +440,4 @@ let initiator_recv_msg_4 a msg4_idx a_si =
       | _ -> error "i_recv_m4: wrong message\n"
   )
   | _ -> error "i_recv_m4: wrong session\n"
+#pop-options
