otway-rees-fixed/OYRS.SecurityProps.fsti
@@ -32,6 +32,30 @@ val principals_and_conv_key_stored_in_auth_server_state:
   (conv_key:bytes) ->
   Type0
 
+/// Ensures that responder, server and conversation key are stored in the initiator state
+val responder_and_server_and_conv_key_stored_in_initiator_state:
+  (initiator:principal) ->
+  (set_state_idx:nat) ->
+  (vv:version_vec) ->
+  (init_state:state_vec) ->
+  (state_session_idx:nat) ->
+  (responder:principal) ->
+  (server:principal) ->
+  (conv_key:bytes) ->
+  Type0
+
+/// Ensures that initiator, server and conversation key are stored in the responder state
+val initiator_and_server_and_conv_key_stored_in_responder_state:
+  (responder:principal) ->
+  (set_state_idx:nat) ->
+  (vv:version_vec) ->
+  (resp_state:state_vec) ->
+  (state_session_idx:nat) ->
+  (initiator:principal) ->
+  (server:principal) ->
+  (conv_key:bytes) ->
+  Type0
+
 /// Ensures secrecy of the generated conversation key for honest principals.
 /// Note: This does not include general secrecy of the conversation key stored
 /// in the states of the initiator and responder, respectively.
@@ -48,6 +72,64 @@ val conv_key_stored_in_auth_server_state_is_secret:
   (requires (fun in_tr ->
     // Stuff stored in state
     principals_and_conv_key_stored_in_auth_server_state server set_state_idx vv server_state state_session_idx initiator responder conv_key /\
+    // State was set before
+    set_state_idx < trace_len in_tr
+  ))
+  (ensures (fun in_tr _ out_tr ->
+    in_tr == out_tr /\
+    (
+      is_unknown_to_attacker_at (trace_len in_tr) conv_key \/
+      (
+        corrupt_id (trace_len in_tr) (P server) \/
+        corrupt_id (trace_len in_tr) (P initiator) \/
+        corrupt_id (trace_len in_tr) (P responder)
+      )
+    )
+  ))
+
+/// Ensures secrecy of the conversation key stored in the initiator state
+val conv_key_stored_in_initiator_state_is_secret:
+  (initiator:principal) ->
+  (set_state_idx:nat) ->
+  (vv:version_vec) ->
+  (init_state:state_vec) ->
+  (state_session_idx:nat) ->
+  (responder:principal) ->
+  (server:principal) ->
+  (conv_key:bytes) ->
+  LCrypto unit (pki oyrs_preds)
+  (requires (fun in_tr ->
+    // Stuff stored in state
+    responder_and_server_and_conv_key_stored_in_initiator_state initiator set_state_idx vv init_state state_session_idx responder server conv_key /\
+    // State was set before
+    set_state_idx < trace_len in_tr
+  ))
+  (ensures (fun in_tr _ out_tr ->
+    in_tr == out_tr /\
+    (
+      is_unknown_to_attacker_at (trace_len in_tr) conv_key \/
+      (
+        corrupt_id (trace_len in_tr) (P server) \/
+        corrupt_id (trace_len in_tr) (P initiator) \/
+        corrupt_id (trace_len in_tr) (P responder)
+      )
+    )
+  ))
+
+/// Ensures secrecy of the conversation key stored in the responder state
+val conv_key_stored_in_responder_state_is_secret:
+  (responder:principal) ->
+  (set_state_idx:nat) ->
+  (vv:version_vec) ->
+  (resp_state:state_vec) ->
+  (state_session_idx:nat) ->
+  (initiator:principal) ->
+  (server:principal) ->
+  (conv_key:bytes) ->
+  LCrypto unit (pki oyrs_preds)
+  (requires (fun in_tr ->
+    // Stuff stored in state
+    initiator_and_server_and_conv_key_stored_in_responder_state responder set_state_idx vv resp_state state_session_idx initiator server conv_key /\
     // State was set before
     set_state_idx < trace_len in_tr
   ))
